proof/DynamicLemmas.thy
@@ -37,123 +37,94 @@ lemma find_firsts_min_in_subset: "f \<in># find_firsts s h v e \<Longrightarrow>
   by (metis set_mset_mono finite_set_mset)
 
 (* Invert single-constructor relations *)
-method elim_Ev = (elim EvFire.cases EvMatch.cases EvGather.cases EvGain.cases; clarsimp)
-method intro_Ev = (intro EvMatches.intros EvMatch.intros EvGain.intros EvGather.intros EvSelect.intros EvConsume.intros)
+method elim_Ev = (elim EvFire.cases EvExec.cases EvMatch.cases EvGather.cases EvConsume.cases EvGain.cases; clarsimp)
+method intro_Ev = (intro EvMatches.intros EvExec.intros EvMatch.intros EvGain.intros EvGather.intros EvSelect.intros EvConsume.intros)
 
 (* trivial *)
-lemma EvFire_new_is_added:
-  "asub | store \<turnstile> rul \<Down> dspent | dnew | store' FIRE \<Longrightarrow>
+lemma new_is_added:
+  "asub | store \<turnstile> rul \<Down> fread | dspent | dnew | store' FIRE \<Longrightarrow>
    dnew \<subseteq># store'"
+  using mset_subset_eq_add_right
+  by (elim EvFire.cases; blast)
+
+
+(* We only spend what we have - trivial *)
+lemma spent_is_subset:
+  "asub | store \<turnstile> rul \<Down> fread | dspent | dnew | store' FIRE \<Longrightarrow>
+   dspent \<subseteq># store"
   by elim_Ev
 
-(*
-(* We only spend what we have - trivial *)
-lemma EvMatches_spent_is_subset:
-  "rn | asub | store | h \<turnstile> matches \<Down> ahas | dspent | h' MATCHES \<Longrightarrow>
-   store_of_used_facts dspent \<subseteq># store"
-  unfolding store_of_used_facts_def
+
+(* We only spend and read what we have - trivial *)
+lemma spent_read_is_subset_EvMatches:
+  "rn | asub | store | h \<turnstile> matches \<Down> fread | dspent | ahas | h' MATCHES \<Longrightarrow>
+   fread \<subseteq># store"
 proof (induct rule: EvMatches.induct)
-  case (EvMatchNil n a s h)
-  then show ?case
-    by (auto simp add: used_facts_empty_def)
-next
   case (EvMatchCons n a s h m ag ds h' ms ag' ds' h'')
   then show ?case
-    apply elim_Ev
-    apply (elim EvConsume.cases)
-     apply (simp add: used_facts_add_def used_facts_empty_def add.commute count_le_replicate_mset_subset_eq subset_mset.le_diff_conv2)
-(*    sledgehammer
-     apply (meson mset_subset_eq_exists_conv subset_mset.order_trans)
-    by (simp add: used_facts_add_def)
-qed
-*)
-    oops
-*)
+    by (elim_Ev; metis EvSelect.cases find_firsts_in_store mset_subset_eqD multiset_filter_subset)
+qed auto
 
-lemma EvFire_spent_is_subset:
-  "asub | store \<turnstile> rul \<Down> dspent | dnew | store' FIRE \<Longrightarrow>
-   store_of_used_facts dspent \<subseteq># store"
+lemma spent_read_is_subset:
+  "asub | store \<turnstile> rul \<Down> fread | dspent | dnew | store' FIRE \<Longrightarrow>
+   fread \<union># dspent \<subseteq># store"
+  using spent_read_is_subset_EvMatches
   by elim_Ev
-
 
 
 (* We only use what we spend *)
 lemma frame_constriction_EvMatches:
-  "rn | asub | store  | h \<turnstile> matches \<Down> ahas | dspent | h' MATCHES \<Longrightarrow>
-   store_of_used_facts dspent \<subseteq># ds' \<Longrightarrow> ds' \<subseteq># store \<Longrightarrow>
-   rn | asub | ds' | h \<turnstile> matches \<Down> ahas | dspent | h' MATCHES"
-unfolding store_of_used_facts_def
+  "rn | asub | store  | h \<turnstile> matches \<Down> fread | dspent | ahas | h' MATCHES \<Longrightarrow>
+   fread \<union># dspent \<subseteq># ds' \<Longrightarrow> ds' \<subseteq># store \<Longrightarrow>
+   rn | asub | ds' | h \<turnstile> matches \<Down> fread | dspent | ahas | h' MATCHES"
 proof (induct arbitrary: ds' rule: EvMatches.induct)
-  case (EvMatchNil n a s h)
-  then show ?case
-    using EvMatches.intros by simp
-next
-  case (EvMatchCons n a s h m ag ds h' ms ag' ds' h'')
-  then show ?case
-    apply -
-    apply (unfold used_facts_add_def)
-    apply (elim EvFire.cases EvMatch.cases EvGather.cases EvGain.cases; clarsimp)
-    apply (elim EvConsume.cases EvSelect.cases; clarsimp)
-       apply (intro_Ev; (rule refl)?; (simp add: used_facts_add_def)?)
-        apply (metis count_inI count_le_replicate_mset_subset_eq le_zero_eq mset_subset_eq_add_left not_gr_zero subseteq_mset_def)
-       apply (metis (no_types, lifting) EvMatchCons.hyps(3) mset_subset_eq_add_right subset_mset.sup.absorb_iff1 subset_mset.sup.bounded_iff)
-      apply (intro_Ev; (rule refl)?; (simp add: used_facts_add_def)?)
-       apply (rule find_firsts_min_in_subset)
-         apply assumption
+  case (EvMatchCons n a s h m f w ag h' ms fs ds ag' h'' fs' ds' ag'')
+  obtain x gather sel con gain where match_is:
+    "m = match x gather sel con gain"
+    using match.exhaust by blast
+  from EvMatchCons match_is have IHrest:
+    "n | a | ds' | h(x := f) \<turnstile> ms \<Down> fs | ds | ag' | h'' MATCHES"
+    by (elim_Ev; metis EvMatchCons.hyps(3) mset_subset_eq_add_right subset_mset.sup.absorb_iff1 subset_mset.sup.bounded_iff)
+  from EvMatchCons match_is  show ?case
+    apply (elim_Ev)
+    apply (elim EvSelect.cases; clarsimp)
+     apply (intro_Ev; (rule refl)?; simp add: IHrest)
+    apply (intro_Ev; (rule refl)?; (simp add: IHrest)?)
+    apply (rule find_firsts_min_in_subset)
+      apply assumption
     using multiset_filter_mono
-        apply blast
-       apply (smt count_inI count_le_replicate_mset_subset_eq find_firsts_in_store le_zero_eq mem_Collect_eq mset_subset_eq_add_left not_gr_zero set_mset_filter subset_mset.order.trans)
-    apply (metis (no_types, lifting) EvMatchCons.hyps(3) mset_subset_eq_add_right subset_mset.sup.absorb_iff1 subset_mset.sup.bounded_iff)
-      apply (intro_Ev; (rule refl)?; (simp add: used_facts_add_def)?)
-    apply (simp add: mset_subset_eqD)
-    using EvMatchCons.hyps(3) subset_mset.sup.boundedI
-    apply blast
-      apply (intro_Ev; (rule refl)?; (simp add: used_facts_add_def)?)
-       apply (rule find_firsts_min_in_subset)
-         apply assumption
-    using multiset_filter_mono
-        apply blast
-       apply (smt count_inI count_le_replicate_mset_subset_eq find_firsts_in_store le_zero_eq mem_Collect_eq mset_subset_eq_add_left not_gr_zero set_mset_filter subset_mset.order.trans)
-    using EvMatchCons.hyps(3) subset_mset.le_supI by blast
-qed
+     apply blast
+    by (metis count_filter_mset find_firsts_in_store not_in_iff)
+qed (auto intro: EvMatches.intros)
 
 lemma frame_constriction:
-  "asub | store  \<turnstile> rul \<Down> dspent | dnew | store' FIRE \<Longrightarrow>
-   asub | store_of_used_facts dspent \<turnstile> rul \<Down> dspent | dnew | (dnew + (facts_retained dspent - facts_consumed dspent))   FIRE"
-  apply elim_Ev
-  using frame_constriction_EvMatches
-  apply (intro EvFire.intros; blast?)
-  apply (unfold store_of_used_facts_def)
-  by (metis add.commute multi_union_self_other_eq subset_mset.add_diff_inverse subset_mset.sup.cobounded1 sup_subset_mset_def)
+  "asub | store  \<turnstile> rul \<Down> fread | dspent | dnew | store' FIRE \<Longrightarrow>
+   asub | (fread \<union># dspent) \<turnstile> rul \<Down> fread | dspent | dnew | (dnew + (fread - dspent))   FIRE"
+  apply (elim EvFire.cases; clarsimp)
+  apply (intro EvFire.intros; assumption?)
+    apply (rule frame_constriction_EvMatches; simp)
+    apply (simp add: spent_read_is_subset_EvMatches)
+  by (simp add: spent_read_is_subset_EvMatches subset_mset.sup_commute sup_subset_mset_def)+
+
 
 (* We only spend visible facts *)
 lemma spend_only_accessible_EvMatches:
-  "rn | asub | store  | h \<turnstile> matches \<Down> ahas | dspent | h' MATCHES  \<Longrightarrow>
-   (\<forall>f \<in># store_of_used_facts dspent. can_see_fact asub f)"
+  "rn | asub | store  | h \<turnstile> matches \<Down> fread | dspent | ahas | h' MATCHES  \<Longrightarrow>
+   (\<forall>f \<in># fread \<union># dspent. can_see_fact asub f)"
 proof (induct rule: EvMatches.induct)
-  case (EvMatchNil n a s h)
+  case (EvMatchCons n a s h m f w ag h' ms fs ds ag' h'' fs' ds' ag'')
   then show ?case
-    by (simp add: store_of_used_facts_def used_facts_add_def used_facts_empty_def)
-next
-  case (EvMatchCons n a s h m ag fw s' h' ms ag' ds' h'')
-  then show ?case
-    apply elim_Ev
-    apply (simp add: store_of_used_facts_def used_facts_add_def used_facts_empty_def)
-    apply (elim EvSelect.cases;
-           clarsimp)
-     apply (elim EvConsume.cases;
-            fastforce simp add: check_gather_def)
-    by (elim EvConsume.cases;
-        clarsimp;
-        smt UnCI check_gather_def find_firsts_in_store mem_Collect_eq set_mset_filter)
-qed
+    apply (elim_Ev; elim EvSelect.cases)
+    using check_gather_def find_firsts_def by auto
+qed auto
 
 lemma spend_only_accessible:
-  "asub | store \<turnstile> rul \<Down> dspent | dnew | store' FIRE \<Longrightarrow>
-   (\<forall>f \<in># store_of_used_facts dspent. can_see_fact asub f)"
+  "asub | store \<turnstile> rul \<Down> fread | dspent | dnew | store' FIRE \<Longrightarrow>
+   (\<forall>f \<in># fread \<union># dspent. can_see_fact asub f)"
   by (elim EvFire.cases; force simp add: spend_only_accessible_EvMatches)
 
 
+(* Helper lemma: if it's not visible, "check_gather" filters it out *)
 lemma check_gather_inaccessible_empty:
   " (\<forall>f \<in># others. \<not>(can_see_fact asub f)) \<Longrightarrow>
   filter_mset (check_gather asub env v ctor pred) others = {#}"
@@ -162,66 +133,55 @@ lemma check_gather_inaccessible_empty:
 
 (* We can always add new facts if they're not visible *)
 lemma store_weaken_inaccessible_EvMatches:
-  "rn | asub | store            | h \<turnstile> matches \<Down> ahas | dspent | h' MATCHES  \<Longrightarrow>
+  "rn | asub | store            | h \<turnstile> matches \<Down> fread | dspent | ahas | h' MATCHES  \<Longrightarrow>
    (\<forall>f \<in># others. \<not>(can_see_fact asub f)) \<Longrightarrow>
-   rn | asub | (store + others) | h \<turnstile> matches \<Down> ahas | dspent | h' MATCHES"
+   rn | asub | (store + others) | h \<turnstile> matches \<Down> fread | dspent | ahas | h' MATCHES"
 proof (induct rule: EvMatches.induct)
   case (EvMatchNil n a s h)
   then show ?case
     using EvMatches.EvMatchNil by blast
 next
-  case (EvMatchCons n a s h m ag fw s' h' ms ag' ds' h'')
+  case (EvMatchCons n a s h m f w ag h' ms fs ds ag' h'' fs' ds' ag'')
   then show ?case
-    apply elim_Ev
-    apply (elim EvSelect.cases)
-     apply (elim EvConsume.cases;
-            clarsimp)
-      apply (intro_Ev;
-            (rule refl)?;
-             simp?;
-             argo EvMatchCons.hyps)+
-    apply (intro_Ev;
-          (rule refl)?;
-          simp?)
+    apply (elim_Ev; elim EvSelect.cases)
+     apply (intro_Ev; (rule refl)?; (simp add: fun_upd_def)?)
      apply (subst check_gather_inaccessible_empty[where others=others];
             simp add: EvSelect.simps)
-    using EvMatchCons.hyps by blast
+    apply (intro_Ev; (rule refl)?; (simp add: fun_upd_def)?)
+    by (subst check_gather_inaccessible_empty[where others=others];
+            simp add: EvSelect.simps)
 qed
 
 lemma store_weaken_inaccessible:
-  "asub |  store           \<turnstile> rul \<Down> dspent | dnew |  store'           FIRE \<Longrightarrow>
+  "asub |  store           \<turnstile> rul \<Down> fread | dspent | dnew |  store'           FIRE \<Longrightarrow>
    (\<forall>f \<in># others. \<not>(can_see_fact asub f)) \<Longrightarrow>
-   asub | (store + others) \<turnstile> rul \<Down> dspent | dnew | (store' + others) FIRE"
+   asub | (store + others) \<turnstile> rul \<Down> fread | dspent | dnew | (store' + others) FIRE"
   apply (elim EvFire.cases; clarsimp)
   apply (intro EvFire.intros)
   using store_weaken_inaccessible_EvMatches
       apply blast
      apply blast
     apply (simp add: subset_mset.add_increasing2)
-   apply (metis ab_semigroup_add_class.add_ac(1) add.commute store_of_used_facts_def subset_mset.add_diff_assoc2 subset_mset.sup.bounded_iff)
+   apply (metis ab_semigroup_add_class.add_ac(1) add.commute  subset_mset.add_diff_assoc2)
   by blast
 
 
 (* auth of new facts is subset of auth of all spent facts *)
 lemma new_auth_gained_from_spent_EvMatches:
-  "rn | asub | store | h \<turnstile> matches \<Down> ahas | dspent | h' MATCHES  \<Longrightarrow>
-  \<forall>a \<in> ahas. \<exists>d \<in># store_of_used_facts dspent. a \<in> fact_by d"
+  "rn | asub | store | h \<turnstile> matches \<Down> fread | dspent | ahas | h' MATCHES  \<Longrightarrow>
+  \<forall>a \<in> ahas. \<exists>d \<in># fread \<union># dspent. a \<in> fact_by d"
 proof (induct rule: EvMatches.induct)
-  case (EvMatchNil n a s h)
-  then show ?case by simp
-next
   case (EvMatchCons n a s h m ag fw s' h' ms ag' ds' h'')
   then show ?case
     by (elim_Ev;
         elim EvSelect.cases;
-        elim EvConsume.cases;
-        clarsimp simp add: store_of_used_facts_def used_facts_add_def used_facts_empty_def;
+        clarsimp;
         blast)
-qed
+qed auto
 
 lemma new_auth_gained_from_spent:
-  "asub | store \<turnstile> rul \<Down> dspent | dnew | store' FIRE \<Longrightarrow>
-  \<forall>f \<in># dnew. \<forall>a \<in> fact_by f. \<exists>d \<in># store_of_used_facts dspent. a \<in> fact_by d"
+  "asub | store \<turnstile> rul \<Down> fread | dspent | dnew | store' FIRE \<Longrightarrow>
+  \<forall>f \<in># dnew. \<forall>a \<in> fact_by f. \<exists>d \<in># fread \<union># dspent. a \<in> fact_by d"
   using new_auth_gained_from_spent_EvMatches
   by (elim EvFire.cases; blast)
 
@@ -237,9 +197,9 @@ fun rule_only_any :: "rule \<Rightarrow> bool" where
 (* This probably isn't true for 'first' selectors, where adding more permissions could make a new minimum visible *)
 (* But if the program only contains any selectors, it is true *)
 lemma auth_weaken_EvMatches:
-  "rn |  asub           | store | h \<turnstile> matches \<Down> ahas | dspent | h' MATCHES  \<Longrightarrow>
+  "rn |  asub           | store | h \<turnstile> matches \<Down> fread | dspent | ahas | h' MATCHES  \<Longrightarrow>
     matches_only_any matches \<Longrightarrow>
-   rn | (asub \<union> others) | store | h \<turnstile> matches \<Down> ahas | dspent | h' MATCHES"
+   rn | (asub \<union> others) | store | h \<turnstile> matches \<Down> fread | dspent | ahas | h' MATCHES"
 proof (induct rule: EvMatches.induct)
 case (EvMatchNil n a s h)
   then show ?case
@@ -255,9 +215,9 @@ next
 qed
 
 lemma auth_weaken:
-  "asub           | store \<turnstile> rul \<Down> dspent | dnew | store' FIRE \<Longrightarrow>
+  "asub           | store \<turnstile> rul \<Down> fread | dspent | dnew | store' FIRE \<Longrightarrow>
     rule_only_any rul \<Longrightarrow>
-  (asub \<union> others) | store \<turnstile> rul \<Down> dspent | dnew | store' FIRE"
+  (asub \<union> others) | store \<turnstile> rul \<Down> fread | dspent | dnew | store' FIRE"
   apply (elim EvFire.cases)
   using auth_weaken_EvMatches
   by (metis EvFire.intros diff_union_cancelL mset_subset_eq_exists_conv rule_only_any.simps union_commute)
@@ -265,9 +225,9 @@ lemma auth_weaken:
 
 (* We can always add new facts if the program only contains 'any' selectors *)
 lemma store_weaken_if_any_EvMatches:
-  "rn | asub |  store            | h \<turnstile> matches \<Down> ahas | dspent | h' MATCHES  \<Longrightarrow>
+  "rn | asub |  store           | h \<turnstile> matches \<Down> fread | dspent | ahas | h' MATCHES  \<Longrightarrow>
     matches_only_any matches \<Longrightarrow>
-   rn | asub | (store + others) | h \<turnstile> matches \<Down> ahas | dspent | h' MATCHES"
+   rn | asub | (store + others) | h \<turnstile> matches \<Down> fread | dspent | ahas | h' MATCHES"
 proof (induct rule: EvMatches.induct)
 case (EvMatchNil n a s h)
   then show ?case
@@ -282,13 +242,13 @@ next
 qed
 
 lemma store_weaken_if_any:
-  "asub |  store            \<turnstile> rul \<Down> dspent | dnew | store' FIRE \<Longrightarrow>
+  "asub |  store           \<turnstile> rul \<Down> fread | dspent | dnew | store' FIRE \<Longrightarrow>
    rule_only_any rul \<Longrightarrow>
-   asub | (store + others) \<turnstile> rul \<Down> dspent | dnew | (store' + others) FIRE"
+   asub | (store + others) \<turnstile> rul \<Down> fread | dspent | dnew | (store' + others) FIRE"
   apply (elim EvFire.cases EvExec.cases; clarsimp)
   apply (intro EvFire.intros EvExec.intros; (rule refl)?; assumption?)
     apply (simp add: store_weaken_if_any_EvMatches)
    apply (simp add: subset_mset.add_increasing2)
-  by (metis add.commute add.left_commute store_of_used_facts_def subset_mset.add_diff_assoc subset_mset.dual_order.trans subset_mset.sup.cobounded1)
+  by (metis add.commute add.left_commute  subset_mset.add_diff_assoc)
 
 end
